Add Expect[Valid|Invalid]AAS helper methods (#215)
Also move helper methods to separate modules, which avoids xUnit warning about them

test/SDK/Client.dfy
@@ -19,35 +19,43 @@ module {:extern "TestClient"} TestClient {
   import RawRSAKeyringDef
   import Materials
   import Client = ESDKClient
-  import Msg = MessageHeader
-  import UTF8
   import Base64
-
-  method EncryptDecryptTest(cmm: CMMDefs.CMM)
-    requires cmm.Valid()
-  {
-    var msg :- expect UTF8.Encode("hello");
-    var keyA :- expect UTF8.Encode("keyA");
-    var valA :- expect UTF8.Encode("valA");
-    var encryptionContext := map[keyA := valA];
-    assert Msg.ValidAAD(encryptionContext) by {
-      // To prove ValidAAD, we need to reveal the definition of ValidAAD:
-      reveal Msg.ValidAAD();
-      // We also need to help the verifier with proving the KVPairsLength is small:
-      calc {
-        Msg.KVPairsLength(encryptionContext);
-        var keys: seq<UTF8.ValidUTF8Bytes> := SetToOrderedSequence<uint8>(encryptionContext.Keys, UInt.UInt8Less);
-        var kvPairsSeq := seq(|keys|, i requires 0 <= i < |keys| => (keys[i], encryptionContext[keys[i]]));
-        2 + Msg.KVPairEntriesLength(kvPairsSeq, 0, |kvPairsSeq|); // 2 bytes for the kvPairsCount field
-        2 + 2 + |keyA| + 2 + |valA|; // 2 bytes required for keyLength and valueLength fields
+  import UTF8
+    
+  module Helpers {
+    import opened StandardLibrary
+    import opened UInt = StandardLibrary.UInt
+    import CMMDefs
+    import DefaultCMMDef
+    import Msg = MessageHeader
+    import UTF8
+    import Client = ESDKClient
+  
+    method EncryptDecryptTest(cmm: CMMDefs.CMM) requires cmm.Valid()
+    {
+      var msg :- expect UTF8.Encode("hello");
+      var keyA :- expect UTF8.Encode("keyA");
+      var valA :- expect UTF8.Encode("valA");
+      var encryptionContext := map[keyA := valA];
+      assert Msg.ValidAAD(encryptionContext) by {
+        // To prove ValidAAD, we need to reveal the definition of ValidAAD:
+        reveal Msg.ValidAAD();
+        // We also need to help the verifier with proving the KVPairsLength is small:
+        calc {
+          Msg.KVPairsLength(encryptionContext);
+          var keys: seq<UTF8.ValidUTF8Bytes> := SetToOrderedSequence<uint8>(encryptionContext.Keys, UInt.UInt8Less);
+          var kvPairsSeq := seq(|keys|, i requires 0 <= i < |keys| => (keys[i], encryptionContext[keys[i]]));
+          2 + Msg.KVPairEntriesLength(kvPairsSeq, 0, |kvPairsSeq|); // 2 bytes for the kvPairsCount field
+          2 + 2 + |keyA| + 2 + |valA|; // 2 bytes required for keyLength and valueLength fields
+        }
+        assert Msg.KVPairsLength(encryptionContext) < UINT16_LIMIT;
       }
-      assert Msg.KVPairsLength(encryptionContext) < UINT16_LIMIT;
+      var e :- expect Client.Encrypt(msg, cmm, Some(encryptionContext), None, None);
+
+      var d :- expect Client.Decrypt(e, cmm);
+
+      expect msg == d;
     }
-    var e :- expect Client.Encrypt(msg, cmm, Some(encryptionContext), None, None);
-
-    var d :- expect Client.Decrypt(e, cmm);
-
-    expect msg == d;
   }
 
   method {:test} HappyPath() {
@@ -58,6 +66,6 @@ module {:extern "TestClient"} TestClient {
     var keyring := new RawRSAKeyringDef.RawRSAKeyring(namespace, name, RSA.PaddingMode.PKCS1, Some(ek), Some(dk));
     var cmm := new DefaultCMMDef.DefaultCMM.OfKeyring(keyring);
 
-    EncryptDecryptTest(cmm);
+    Helpers.EncryptDecryptTest(cmm);
   }
 }
